src/QueryStructure/Automation/Constraints/ForeignKeyAutomation.v
@@ -20,12 +20,11 @@ Ltac foreignToQuery :=
     | [ |- context[{ b' | decides b' (ForeignKey_P ?AttrID ?AttrID' ?tupmap ?n (@GetUnConstrRelation ?qs_schema ?or ?TableID))}] ]
       =>
       let H' := fresh in
-      pose (@refine_constraint_check_into_query
-                        qs_schema TableID
-                        (fun tup : Tuple => GetAttribute n AttrID = tupmap (GetAttribute tup AttrID')) or _) as H';
-        unfold QSGetNRelSchemaHeading in H';
-        simpl in *;
-        pose_string_hyps; pose_heading_hyps;
-        fold_string_hyps_in H'; fold_heading_hyps_in H';
-        setoid_rewrite H'; simplify with monad laws; cbv beta; simpl; clear H'
+      let H' :=
+      eval simpl in (@refine_constraint_check_into_query
+                       qs_schema TableID
+                       (fun tup : RawTuple => GetAttributeRaw n AttrID = tupmap (GetAttributeRaw tup AttrID')) or _) in
+          pose_string_hyps; pose_heading_hyps;
+                    (* fold_string_hyps_in H'; fold_heading_hyps_in H'; *)
+                    setoid_rewrite H'; simplify with monad laws; cbv beta; simpl
   end.
