src/QueryStructure/Implementation/Operations/General/QueryRefinements.v
@@ -812,7 +812,7 @@ Qed. *)
 Lemma DropQSConstraintsQuery_In {A} :
   forall qs_schema qs R bod,
     @Query_In A qs_schema qs R bod =
-    UnConstrQuery_In (DropQSConstraints qs) (ibound (indexb R)) bod.
+    UnConstrQuery_In (DropQSConstraints qs) R bod.
 Proof.
   intros; unfold Query_In, UnConstrQuery_In, GetRelation, GetUnConstrRelation,
           DropQSConstraints; rewrite <- ith_imap2.
@@ -822,7 +822,7 @@ Qed.
 Lemma DropQSConstraintsQuery_In_UnderBinder {A B} :
   forall qs_schema qs R bod,
     (fun b : B => @Query_In A qs_schema qs R (bod b)) =
-    (fun b : B => UnConstrQuery_In (DropQSConstraints qs) (ibound (indexb R)) (bod b)).
+    (fun b : B => UnConstrQuery_In (DropQSConstraints qs) R (bod b)).
 Proof.
     intros; unfold Query_In, UnConstrQuery_In, GetRelation, GetUnConstrRelation,
           DropQSConstraints; rewrite <- ith_imap2.
